TAPLFormalization/BigStep.lean
@@ -3,48 +3,48 @@ import TAPLFormalization.Semantics
 import TAPLFormalization.SemanticsTheorems
 
 inductive BigStep : Term → Term → Prop where
-  | value : IsValue v → BigStep v v
-  | ifTrue : IsValue v → BigStep t₁ .trueV → BigStep t₂ v
+  | value : v.IsValue → BigStep v v
+  | ifTrue : v.IsValue → BigStep t₁ .trueV → BigStep t₂ v
     → BigStep (.ifThenElse t₁ t₂ t₃) v
-  | ifFalse : IsValue v → BigStep t₁ .falseV → BigStep t₃ v
+  | ifFalse : v.IsValue → BigStep t₁ .falseV → BigStep t₃ v
     → BigStep (.ifThenElse t₁ t₂ t₃) v
-  | succ : IsNumericValue v → BigStep t₁ v → BigStep (.succ t₁) (.succ v)
+  | succ : v.IsNumericValue → BigStep t₁ v → BigStep (.succ t₁) (.succ v)
   | predZero : BigStep t₁ .zero → BigStep (.pred t₁) .zero
-  | predSucc : IsNumericValue v → BigStep t₁ (.succ v) → BigStep (.pred t₁) v
+  | predSucc : v.IsNumericValue → BigStep t₁ (.succ v) → BigStep (.pred t₁) v
   | isZeroZero : BigStep t₁ .zero → BigStep (.isZero t₁) .trueV
-  | isZeroSucc : IsNumericValue v → BigStep t₁ (.succ v) → BigStep (.isZero t₁) .falseV
+  | isZeroSucc : v.IsNumericValue → BigStep t₁ (.succ v) → BigStep (.isZero t₁) .falseV
 
-lemma smallStep_preserves_bigStep : IsValue v → t ~> t' → BigStep t' v → BigStep t v := by
+lemma smallStep_preserves_bigStep : v.IsValue → t ~> t' → BigStep t' v → BigStep t v := by
   intro v_value t_st_t' t'_bigst_v
   induction t' generalizing t v <;>
-    grind [BigStep, SmallStep, IsValue, IsNumericValue]
+    grind [BigStep, SmallStep, Term.IsValue, Term.IsNumericValue]
 
-lemma bigStep_of_smallSteps : IsValue v → t ~>* v → BigStep t v := by
+lemma bigStep_of_smallSteps : v.IsValue → t ~>* v → BigStep t v := by
   intro v_value t_sts_v
   induction t_sts_v <;> grind [BigStep, smallStep_preserves_bigStep]
 
-lemma smallSteps_of_bigStep : IsValue v → BigStep t v → t ~>* v := by
+lemma smallSteps_of_bigStep : v.IsValue → BigStep t v → t ~>* v := by
   intro v_value t_bigst_v
   induction t_bigst_v
   case value => constructor
   case ifTrue v_value t₁_bst_trueV t₂_bst_v ih_trueV ih_v =>
-    rename_i v t₁ t₂ t₃ _
+    rename_i t₁ t₂ v t₃ _
     let t₁_sts_trueV := ih_trueV (by constructor)
     let t₂_sts_v := ih_v v_value
-    let sts₁ : t₁.ifThenElse t₂ t₃ ~>* .ifThenElse .trueV t₂ t₃ := smallSteps_in_context
-      (.ifThenElse · t₂ t₃) SmallStep.If t₁_sts_trueV
-    let sts₂ : t₁.ifThenElse t₂ t₃ ~>* t₂ := SmallSteps.trans'.trans sts₁ .IfTrue
-    exact SmallSteps.trans.trans sts₂ t₂_sts_v
+    let sts₁ : t₁.ifThenElse t₂ t₃ ~>* .ifThenElse .trueV t₂ t₃ := ReflTransGen'.lift
+      (Term.ifThenElse · t₂ t₃) SmallStep.If t₁_sts_trueV
+    let sts₂ : t₁.ifThenElse t₂ t₃ ~>* t₂ := ReflTransGen'.trans' sts₁ .IfTrue
+    exact ReflTransGen'.trans sts₂ t₂_sts_v
   case ifFalse v_value t₁_bigst_falseV t₂_bst_v ih_falseV ih_v =>
-    rename_i v t₁ t₂ t₃ _
+    rename_i t₁ t₂ v t₃ _
     let t₁_sts_falseV := ih_falseV (by constructor)
     let t₂_sts_v := ih_v v_value
-    let sts₁ : t₁.ifThenElse t₃ t₂ ~>* .ifThenElse .falseV t₃ t₂ := smallSteps_in_context
-      (.ifThenElse · t₃ t₂) SmallStep.If t₁_sts_falseV
-    let sts₂ : t₁.ifThenElse t₃ t₂ ~>* t₂ := SmallSteps.trans'.trans sts₁ .IfFalse
-    exact SmallSteps.trans.trans sts₂ t₂_sts_v
+    let sts₁ : t₁.ifThenElse t₃ t₂ ~>* .ifThenElse .falseV t₃ t₂ := ReflTransGen'.lift
+      (Term.ifThenElse · t₃ t₂) SmallStep.If t₁_sts_falseV
+    let sts₂ : t₁.ifThenElse t₃ t₂ ~>* t₂ := ReflTransGen'.trans' sts₁ .IfFalse
+    exact ReflTransGen'.trans sts₂ t₂_sts_v
   case succ v_value t_bst_v ih =>
-    apply smallSteps_in_context .succ SmallStep.Succ
+    apply ReflTransGen'.lift Term.succ SmallStep.Succ
     apply ih
     cases v_value
     rename_i v_nv
@@ -52,29 +52,29 @@ lemma smallSteps_of_bigStep : IsValue v → BigStep t v → t ~>* v := by
     constructor
     assumption
   case predZero t_st_zero ih =>
-    let sts₁ := smallSteps_in_context .pred SmallStep.Pred
+    let sts₁ := ReflTransGen'.lift Term.pred SmallStep.Pred
       (ih (by repeat constructor))
-    apply SmallSteps.trans'.trans sts₁
+    apply ReflTransGen'.trans' sts₁
     constructor
   case predSucc v_nv t_bst_v_succ ih =>
-    let sts₁ := smallSteps_in_context .pred SmallStep.Pred
+    let sts₁ := ReflTransGen'.lift Term.pred SmallStep.Pred
       (ih (by constructor; constructor; assumption))
-    apply SmallSteps.trans'.trans sts₁
+    apply ReflTransGen'.trans' sts₁
     constructor
     assumption
   case isZeroZero t_bst_zero ih =>
-    let sts₁ := smallSteps_in_context .isZero SmallStep.IsZero
+    let sts₁ := ReflTransGen'.lift Term.isZero SmallStep.IsZero
       (ih (by repeat constructor))
-    apply SmallSteps.trans'.trans sts₁
+    apply ReflTransGen'.trans' sts₁
     constructor
   case isZeroSucc v_nv t_bst_v_succ ih =>
-    let sts₁ := smallSteps_in_context .isZero SmallStep.IsZero
+    let sts₁ := ReflTransGen'.lift Term.isZero SmallStep.IsZero
       (ih (by constructor; constructor; assumption))
-    apply SmallSteps.trans'.trans sts₁
+    apply ReflTransGen'.trans' sts₁
     constructor
     assumption
 
-theorem bigStep_iff_smallSteps : IsValue v → (BigStep t v ↔ t ~>* v) := by
+theorem bigStep_iff_smallSteps : v.IsValue → (BigStep t v ↔ t ~>* v) := by
   intro v_value
   constructor
   · exact smallSteps_of_bigStep v_value
