TAPLFormalization/Common.lean
@@ -1,0 +1,22 @@
+import Mathlib.Logic.Relation
+
+inductive ReflTransGen' (r : α → α → Prop) : α → α → Prop
+  | refl : ReflTransGen' r a a
+  | tail : r a b → ReflTransGen' r b c → ReflTransGen' r a c
+
+lemma ReflTransGen'.single (h : r a b) : ReflTransGen' r a b := .tail h .refl
+
+theorem ReflTransGen'.trans (hab : ReflTransGen' r a b) (hbc : ReflTransGen' r b c) :
+  ReflTransGen' r a c := by
+  induction hab with
+  | refl => assumption
+  | tail r rs ih => exact tail r (ih hbc)
+
+theorem ReflTransGen'.trans' (hab : ReflTransGen' r a b) (hbc : r b c) :
+  ReflTransGen' r a c := trans hab (.single hbc)
+
+theorem ReflTransGen'.lift (f : α → β) (h : ∀ {a b}, r a b → p (f a) (f b))
+  (hab : ReflTransGen' r a b) : ReflTransGen' p (f a) (f b) := by
+  induction hab with
+  | refl => constructor
+  | tail r rs ih => exact .tail (h r) ih
