TAPLFormalization/Wrong.lean
@@ -1,0 +1,156 @@
+import TAPLFormalization.Semantics
+import TAPLFormalization.SemanticsTheorems
+
+import Mathlib.Tactic.DefEqTransformations
+
+inductive TermWrong
+  | wrong : TermWrong
+  | trueV : TermWrong
+  | falseV : TermWrong
+  | zero : TermWrong
+  | ifThenElse : TermWrong → TermWrong → TermWrong → TermWrong
+  | succ : TermWrong → TermWrong
+  | pred : TermWrong → TermWrong
+  | isZero : TermWrong → TermWrong
+
+def embed : Term → TermWrong
+  | .trueV => .trueV
+  | .falseV => .falseV
+  | .zero => .zero
+  | .ifThenElse t₁ t₂ t₃ => .ifThenElse (embed t₁) (embed t₂) (embed t₃)
+  | .succ t => .succ (embed t)
+  | .pred t => .pred (embed t)
+  | .isZero t => .isZero (embed t)
+
+inductive TermWrong.IsNumericValue : TermWrong → Prop
+  | zero : IsNumericValue .zero
+  | succ : IsNumericValue t → IsNumericValue (.succ t)
+
+inductive TermWrong.IsValue : TermWrong → Prop
+  | trueV : IsValue .trueV
+  | falseV : IsValue .falseV
+  | numericV : IsNumericValue t → IsValue t
+
+lemma embed_preserves_nv : t.IsNumericValue → (embed t).IsNumericValue := by
+  intro t_nv
+  induction t_nv <;> constructor
+  assumption
+
+inductive BadNat : TermWrong → Prop
+  | trueV : BadNat .trueV
+  | falseV : BadNat .falseV
+  | wrong : BadNat .wrong
+
+inductive BadBool : TermWrong → Prop
+  | nv : t.IsNumericValue → BadBool t
+  | wrong : BadBool .wrong
+
+inductive SmallStep' : TermWrong → TermWrong → Prop
+  | IfTrue : SmallStep' (.ifThenElse .trueV t₂ t₃) t₂
+  | IfFalse : SmallStep' (.ifThenElse .falseV t₂ t₃) t₃
+  | If : SmallStep' t₁ t₂ → SmallStep' (.ifThenElse t₁ a b) (.ifThenElse t₂ a b)
+  | Succ :  SmallStep' t₁ t₂ → SmallStep' (.succ t₁) (.succ t₂)
+  | PredZero : SmallStep' (.pred .zero) .zero
+  | PredSucc : nv.IsNumericValue → SmallStep' (.pred (.succ nv)) nv
+  | Pred : SmallStep' t₁ t₂ → SmallStep' (.pred t₁) (.pred t₂)
+  | IsZeroZero : SmallStep' (.isZero .zero) .trueV
+  | IsZeroSucc : nv.IsNumericValue → SmallStep' (.isZero (.succ nv)) .falseV
+  | IsZero : SmallStep' t₁ t₂ → SmallStep' (.isZero t₁) (.isZero t₂)
+  | IfWrong : BadBool t₁ → SmallStep' (.ifThenElse t₁ t₂ t₃) .wrong
+  | SuccWrong : BadNat t → SmallStep' (.succ t) .wrong
+  | PredWrong : BadNat t → SmallStep' (.pred t) .wrong
+  | IsZeroWrong : BadNat t → SmallStep' (.isZero t) .wrong
+
+abbrev SmallSteps' := ReflTransGen' SmallStep'
+
+def Stuck (t : Term) : Prop := isNF t ∧ ¬t.IsValue
+
+def GetsStuck (t : Term) : Prop := ∃ t', t ~>* t' ∧ Stuck t'
+
+lemma gets_wrong_if_stuck : Stuck t → SmallSteps' (embed t) .wrong := by
+  rintro ⟨t_NF, t_not_value⟩
+  induction t <;> try grind [Term.IsValue, Term.IsNumericValue]
+  all_goals rw [embed]
+  case ifThenElse c t e ih_c ih_t ih_e =>
+    have c_NF : isNF c := by
+      intro c' c_st_c'
+      apply t_NF
+      apply SmallStep.If
+      assumption
+    by_cases h : c.IsValue
+    case pos =>
+      cases h with
+      | trueV => cases t_NF t .IfTrue
+      | falseV => cases t_NF e .IfFalse
+      | numericV c_nv =>
+        let c_bb := BadBool.nv (embed_preserves_nv c_nv)
+        apply ReflTransGen'.single
+        constructor
+        assumption
+    case neg =>
+      let sts₁ := ReflTransGen'.lift (TermWrong.ifThenElse · (embed t) (embed e)) SmallStep'.If (ih_c c_NF h)
+      beta_reduce at sts₁
+      apply ReflTransGen'.trans' sts₁
+      constructor
+      exact BadBool.wrong
+  case succ t ih =>
+    have t_NF : isNF t := by
+      intro t' t_st_t'
+      apply t_NF
+      constructor
+      assumption
+    by_cases h : t.IsValue
+    case pos =>
+      cases h <;> try (apply ReflTransGen'.single; repeat constructor)
+      rename_i t_nv
+      cases t_not_value (.numericV (.succ t_nv))
+    case neg =>
+      let sts₁ := ReflTransGen'.lift TermWrong.succ SmallStep'.Succ (ih t_NF h)
+      apply ReflTransGen'.trans' sts₁
+      constructor
+      exact BadNat.wrong
+  case pred t ih =>
+    have t_NF : isNF t := by
+      intro t' t_st_t'
+      apply t_NF
+      constructor
+      assumption
+    rename_i t_pred_NF
+    by_cases h : t.IsValue
+    case pos =>
+      cases h <;> try (apply ReflTransGen'.single; repeat constructor)
+      suffices h : False by contradiction
+      rename_i t_nv
+      cases t_nv
+      · cases t_pred_NF _ .PredZero
+      · cases t_pred_NF _ (.PredSucc (by assumption))
+    case neg =>
+      let sts₁ := ReflTransGen'.lift TermWrong.pred SmallStep'.Pred (ih t_NF h)
+      apply ReflTransGen'.trans' sts₁
+      constructor
+      exact BadNat.wrong
+  case isZero t ih =>
+    have t_NF : isNF t := by
+      intro t' t_st_t'
+      apply t_NF
+      constructor
+      assumption
+    rename_i t_pred_NF
+    by_cases h : t.IsValue
+    case pos =>
+      cases h <;> try (apply ReflTransGen'.single; repeat constructor)
+      suffices h : False by contradiction
+      rename_i t_nv
+      cases t_nv
+      · cases t_pred_NF _ .IsZeroZero
+      · cases t_pred_NF _ (.IsZeroSucc (by assumption))
+    case neg =>
+      let sts₁ := ReflTransGen'.lift TermWrong.isZero SmallStep'.IsZero (ih t_NF h)
+      apply ReflTransGen'.trans' sts₁
+      constructor
+      exact BadNat.wrong
+
+theorem getsStuck_iff_gets_wrong : GetsStuck t ↔ SmallSteps' (embed t) .wrong := by
+  constructor
+  · sorry
+  · sorry
